coq/ZF/Meta/Test/Axiom/Choice.v
@@ -13,7 +13,7 @@ Require Import ZF.Meta.Decl.Axiom.Choice.
 Proposition Choice : HasTyDeclT (Choice.env) Choice.
 Proof.
   apply HasTyAll, HasTyEx, HasTyAnd.
-  - apply HasTyIdentT with (d:=FunctionOn). 1: reflexivity.
+  - apply HasTyIdentT with [TySet;TySet]. 1: reflexivity.
     apply HasTyTsCons.
     + apply (HasTyVar _ _ _ TySet). reflexivity.
     + apply HasTyTsCons.
@@ -24,10 +24,10 @@ Proof.
     + apply HasTyImp.
       * apply HasTyNotEq.
         -- apply (HasTyVar _ _ _ TySet). reflexivity.
-        -- apply HasTyIdentT with (d:=empty). 1: reflexivity.
+        -- apply HasTyIdentT with []. 1: reflexivity.
            apply HasTyTsNil.
       * apply HasTyElem.
-        -- apply HasTyIdentT with (d:=eval). 1: reflexivity.
+        -- apply HasTyIdentT with [TySet;TySet]. 1: reflexivity.
            apply HasTyTsCons.
            ++ apply (HasTyVar _ _ _ TySet). reflexivity.
            ++ apply HasTyTsCons.
