coq/ZF/Meta/Test/Axiom/Continuum.v
@@ -15,20 +15,20 @@ Proposition CH : HasTyDeclT (Continuum.env) CH.
 Proof.
   (* Proof by Hermes + gpt 5.5                                                  *)
   apply HasTyEqual.
-  - apply HasTyIdentT with (d:=card). 1: reflexivity.
+  - apply HasTyIdentT with [TySet]. 1: reflexivity.
     apply HasTyTsCons.
-    + apply HasTyIdentT with (d:=power). 1: reflexivity.
+    + apply HasTyIdentT with [TySet]. 1: reflexivity.
       apply HasTyTsCons.
-      * apply HasTyIdentT with (d:=omega). 1: reflexivity.
+      * apply HasTyIdentT with []. 1: reflexivity.
         apply HasTyTsNil.
       * apply HasTyTsNil.
     + apply HasTyTsNil.
-  - apply HasTyIdentT with (d:=eval). 1: reflexivity.
+  - apply HasTyIdentT with [TyClass;TySet]. 1: reflexivity.
     apply HasTyTsCons.
-    + apply HasTyIdentT with (d:=Aleph). 1: reflexivity.
+    + apply HasTyIdentT with []. 1: reflexivity.
       apply HasTyTsNil.
     + apply HasTyTsCons.
-      * apply HasTyIdentT with (d:=one). 1: reflexivity.
+      * apply HasTyIdentT with []. 1: reflexivity.
         apply HasTyTsNil.
       * apply HasTyTsNil.
 Qed.
@@ -37,30 +37,30 @@ Proposition GCH : HasTyDeclT (Continuum.env) GCH.
 Proof.
   (* Proof by Hermes + gpt 5.5                                                  *)
   apply HasTyAll, HasTyImp.
-  - apply HasTyIdentT with (d:=Ordinal). 1: reflexivity.
+  - apply HasTyIdentT with [TySet]. 1: reflexivity.
     apply HasTyTsCons.
     + apply (HasTyVar _ _ _ TySet). reflexivity.
     + apply HasTyTsNil.
   - apply HasTyEqual.
-    + apply HasTyIdentT with (d:=card). 1: reflexivity.
+    + apply HasTyIdentT with [TySet]. 1: reflexivity.
       apply HasTyTsCons.
-      * apply HasTyIdentT with (d:=power). 1: reflexivity.
+      * apply HasTyIdentT with [TySet]. 1: reflexivity.
         apply HasTyTsCons.
-        -- apply HasTyIdentT with (d:=eval). 1: reflexivity.
+        -- apply HasTyIdentT with [TyClass;TySet]. 1: reflexivity.
            apply HasTyTsCons.
-           ++ apply HasTyIdentT with (d:=Aleph). 1: reflexivity.
+           ++ apply HasTyIdentT with []. 1: reflexivity.
               apply HasTyTsNil.
            ++ apply HasTyTsCons.
               ** apply (HasTyVar _ _ _ TySet). reflexivity.
               ** apply HasTyTsNil.
         -- apply HasTyTsNil.
       * apply HasTyTsNil.
-    + apply HasTyIdentT with (d:=eval). 1: reflexivity.
+    + apply HasTyIdentT with [TyClass;TySet]. 1: reflexivity.
       apply HasTyTsCons.
-      * apply HasTyIdentT with (d:=Aleph). 1: reflexivity.
+      * apply HasTyIdentT with []. 1: reflexivity.
         apply HasTyTsNil.
       * apply HasTyTsCons.
-        -- apply HasTyIdentT with (d:=succ). 1: reflexivity.
+        -- apply HasTyIdentT with [TySet]. 1: reflexivity.
            apply HasTyTsCons.
            ++ apply (HasTyVar _ _ _ TySet). reflexivity.
            ++ apply HasTyTsNil.
@@ -72,14 +72,14 @@ Proof.
   (* Proof by Hermes + gpt 5.5                                                  *)
   split.
   - apply HasTyImp.
-    + apply HasTyIdentT with (d:=Decl.Axiom.Continuum.GCH). 1: reflexivity.
+    + apply HasTyIdentT with []. 1: reflexivity.
       apply HasTyTsNil.
-    + apply HasTyIdentT with (d:=Decl.Axiom.Continuum.CH). 1: reflexivity.
+    + apply HasTyIdentT with []. 1: reflexivity.
       apply HasTyTsNil.
   - apply HasTyHoleP.
     apply HasTyImp.
-    + apply HasTyIdentT with (d:=Decl.Axiom.Continuum.GCH). 1: reflexivity.
+    + apply HasTyIdentT with []. 1: reflexivity.
       apply HasTyTsNil.
-    + apply HasTyIdentT with (d:=Decl.Axiom.Continuum.CH). 1: reflexivity.
+    + apply HasTyIdentT with []. 1: reflexivity.
       apply HasTyTsNil.
 Qed.
