coq/ZF/Meta/Test/Class/Incl.v
@@ -143,7 +143,7 @@ Proposition ReflCheck : HasTyT env Ctx.empty Refl TyProp.
 Proof.
   (* Proof by Hermes + gpt 5.5                                                  *)
   apply HasTyAll.
-  apply HasTyIdentT with (d:=Incl). 1: reflexivity.
+  apply HasTyIdentT with [TyClass;TyClass]. 1: reflexivity.
   apply HasTyTsCons.
   - apply (HasTyVar _ _ _ TyClass). reflexivity.
   - apply HasTyTsCons.
